cava/monad-examples/AdderTree.v
@@ -21,10 +21,11 @@
 
 From Coq Require Import Bool.Bool.
 From Coq Require Import Ascii String.
-From Coq Require Import Vector.
-From Coq Require Import Bool.Bvector.
 From Coq Require Arith.PeanoNat.
 Require Import Omega.
+
+From Coq Require Import Lists.List.
+Import ListNotations.
 
 Require Import ExtLib.Structures.Monads.
 
@@ -34,56 +35,51 @@ Require Import Cava.Monad.Cava.
 Require Import Cava.Monad.Combinators.
 Require Import Cava.Monad.UnsignedAdders.
 
-Local Open Scope vector_scope.
 Set Implicit Arguments.
 
-Definition to_n_plus_n {a n} (v : Vector.t a (2*n)) : Vector.t a (n + n).
-Proof.
-  intros. simpl in v. rewrite <- plus_n_O in v. apply v.
-Defined.
+Definition v0 := nat_to_list_bits_sized 8  4.
+Definition v1 := nat_to_list_bits_sized 8 17.
+Definition v2 := nat_to_list_bits_sized 8  6.
+Definition v3 := nat_to_list_bits_sized 8  3.
 
-Definition halve' {n a} (v : Vector.t a (n+n)) : Vector.t a n * Vector.t a n :=
-  splitat n v.
+Definition halve {A} (l : list A) : list A * list A :=
+  let mid := (length l) / 2 in
+  (firstn mid l, skipn mid l).
 
-Definition v0 := nat_to_bitvec_sized 8  4.
-Definition v1 := nat_to_bitvec_sized 8 17.
-Definition v2 := nat_to_bitvec_sized 8  6.
-Definition v3 := nat_to_bitvec_sized 8  3.
-
-Definition v0_3 : Vector.t (Bvector 8) (2+2) := [v0; v1; v2; v3].
-(* Compute halve' v0_3. *)
-
-Definition halve {n a} (v : Vector.t a (2*n)) : Vector.t a n * Vector.t a n :=
-  halve' (to_n_plus_n v).
-
-Fixpoint adderTree {m bit} `{Cava m bit} (n s : nat) (v : Vector.t (Vector.t bit s) (2^(n+1))) : m (Vector.t bit s) :=
-  match n, v with
-  | O, v2 => unsignedAdd s (hd v2) (hd (tl v2))
-  | S n', vR => let '(vL, vH) := halve vR in
-                aS <- adderTree n' vL ;;
-                bS <- adderTree n' vH ;;
-                sum <- unsignedAdd s aS bS ;;
-                ret sum
+Fixpoint adderTree {m bit} `{Cava m bit} (n s : nat) (v: list (list bit)) : m (list bit) :=
+  match n with
+  | O => match v with
+         | [a; b] => unsignedAdd s a b
+         | _ => ret [] (* Error case *)
+         end
+  | S n' => let '(vL, vH) := halve v in
+            aS <- adderTree n' s vL ;;
+            bS <- adderTree n' s vH ;;
+            sum <- unsignedAdd s aS bS ;;
+            ret sum
   end.
  
 (* An adder tree with 2 inputs each of 8 bits in size. *)
 
-Definition adderTree2_8 {m bit} `{Cava m bit} (v : Vector.t (Vector.t bit 8) 2) : m (Vector.t bit 8)
-  := adderTree 0 v.
+Definition adderTree2_8 {m bit} `{Cava m bit} (v : list (list bit)) : m (list bit)
+  := adderTree 0 8 v.
 
-Definition v2_8 : Vector.t (Bvector 8) 2 := [v0; v1].
-Definition v0_plus_v1 : Bvector 8 := combinational (adderTree2_8 v2_8).
-Compute v0_plus_v1.
-
-Example v0_plus_v1_ex : bitvec_to_nat v0_plus_v1 = 21.
+Definition v0_v1 := [v0; v1].
+Definition v0_plus_v1 : list bool := combinational (adderTree2_8 v0_v1).
+Example sum_vo_v1 : list_bits_to_nat v0_plus_v1 = 21.
 Proof. reflexivity. Qed.
 
 (* An adder tree with 4 inputs each of 8 bits in size. *)
 
-Definition adderTree4_8 {m bit} `{Cava m bit} (v : Vector.t (Vector.t bit 8) 4) : m (Vector.t bit 8)
-  := adderTree 1 v.
+Definition adderTree4_8 {m bit} `{Cava m bit} (v : list (list bit)) : m (list bit)
+  := adderTree 1 8 v.
 
-Definition adder_tree4_8_top : state CavaState (Vector.t N 8) :=
+Definition v0_v1_v2_v3 := [v0; v1; v2; v3].
+Definition adderTree4_8_v0_v1_v2_v3 : list bool := combinational (adderTree4_8 v0_v1_v2_v3).
+Example sum_v0_v1_v2_v3 : list_bits_to_nat (combinational (adderTree4_8 v0_v1_v2_v3)) = 30.
+Proof. reflexivity. Qed.
+
+Definition adder_tree4_8_top : state CavaState (list N) :=
   setModuleName "adder_tree4_8" ;;
   a <- inputVectorTo0 8 "a" ;;
   b <- inputVectorTo0 8 "b" ;;
@@ -94,15 +90,4 @@ Definition adder_tree4_8_top : state CavaState (Vector.t N 8) :=
 
 Definition adder_tree4_8Netlist := makeNetlist adder_tree4_8_top.
 
-Definition v4_8 : Vector.t (Bvector 8) (2^(1+1)) := [v0; v1; v2; v3].
-
-Definition adderTree4_8_sim : ident (Vector.t bool 8) := adderTree4_8 v4_8.
-
-(*
-Compute (combinational adderTree4_8_sim).
-*)
-
-(* This computation causes Coq to loop.
-Compute (combinational adderTree4_8_sim).
-*)
 
