cava/monad-examples/UnsignedAdder.v
@@ -17,7 +17,6 @@
 From Coq Require Import Bool.Bool.
 From Coq Require Import Ascii String.
 From Coq Require Import Lists.List.
-From Coq Require Import Vector.
 From Coq Require Import ZArith.
 Import ListNotations.
 
@@ -86,11 +85,9 @@ Definition adder8Top :=
   setModuleName "adder8" ;;
   av <- inputVectorTo0 8 "a" ;;
   bv <- inputVectorTo0 8 "b" ;;
-  let a := Vector.to_list av in
-  let b := Vector.to_list bv in
   cin <- inputBit "cin" ;;
-  '(sum, cout) <- unsignedAdder cin (combine a b) ;;
-  outputVectorTo0 (length sum) (Vector.of_list sum) "sum" ;;
+  '(sum, cout) <- unsignedAdder cin (combine av bv) ;;
+  outputVectorTo0 (length sum) sum "sum" ;;
   outputBit "cout" cout.
 
 Definition adder8Netlist := makeNetlist adder8Top.
